HOL/DataStrs/Mapping.thy
@@ -2,16 +2,13 @@ theory Mapping
 imports "../Auto2_Main"
 begin
 
-setup {* add_rewrite_rule @{thm map_of.simps(1)} *}
-theorem map_of2 [rewrite]:
-  "map_of (p # ps) x = (if x = fst p then Some (snd p) else map_of ps x)" by simp
-
 datatype ('a, 'b) map = Map "'a \<Rightarrow> 'b option"
+
 fun meval :: "('a, 'b) map \<Rightarrow> 'a \<Rightarrow> 'b option" ("_\<langle>_\<rangle>" [90]) where
   "(Map f) \<langle>h\<rangle> = f h"
 setup {* add_rewrite_rule @{thm meval.simps} *}
 
-theorem meval_ext: "\<forall>x. M\<langle>x\<rangle> = N\<langle>x\<rangle> \<Longrightarrow> M = N"
+lemma meval_ext: "\<forall>x. M\<langle>x\<rangle> = N\<langle>x\<rangle> \<Longrightarrow> M = N"
   apply (cases M) apply (cases N) by auto
 setup {* add_backward_prfstep_cond @{thm meval_ext} [with_filt (order_filter "M" "N")] *}
 
@@ -19,145 +16,129 @@ definition empty_map :: "('a, 'b) map" where
   "empty_map = Map (\<lambda>x. None)"
 setup {* add_rewrite_rule @{thm empty_map_def} *}
 
-definition update_map ::
-  "('a, 'b) map \<Rightarrow> 'a \<Rightarrow> 'b \<Rightarrow> ('a ,'b) map" (" _ { _ \<rightarrow> _ }" [89,90,90] 90) where
-  "update_map M k v = Map (\<lambda>x. if x = k then Some v else M\<langle>x\<rangle>)"
+definition update_map :: "('a, 'b) map \<Rightarrow> 'a \<Rightarrow> 'b \<Rightarrow> ('a ,'b) map" (" _ { _ \<rightarrow> _ }" [89,90,90] 90) where
+  "M {k \<rightarrow> v} = Map (\<lambda>x. if x = k then Some v else M\<langle>x\<rangle>)"
 setup {* add_rewrite_rule @{thm update_map_def} *}
 
 definition delete_map :: "'a \<Rightarrow> ('a, 'b) map \<Rightarrow> ('a, 'b) map" where
   "delete_map k M = Map (\<lambda>x. if x = k then None else M\<langle>x\<rangle>)"
 setup {* add_rewrite_rule @{thm delete_map_def} *}
 
-section {* map_of_alist *}
+section {* Map from an AList *}
 
-definition map_of_alist :: "('a \<times> 'b) list \<Rightarrow> ('a, 'b) map" where
-  "map_of_alist xs = Map (map_of xs)"
-setup {* add_rewrite_rule @{thm map_of_alist_def} *}
-
-theorem map_of_alist_simps [rewrite]:
+fun map_of_alist :: "('a \<times> 'b) list \<Rightarrow> ('a, 'b) map" where
   "map_of_alist [] = empty_map"
-  "map_of_alist (x # xs) = update_map (map_of_alist xs) (fst x) (snd x)" by auto2+
-setup {* del_prfstep_thm @{thm map_of_alist_def} *}
+| "map_of_alist (x # xs) = (map_of_alist xs) {fst x \<rightarrow> snd x}"
+setup {* fold add_rewrite_rule @{thms map_of_alist.simps} *}
 
-theorem map_of_alist_nil [rewrite]:
-  "x \<notin> set (map fst ys) \<Longrightarrow> (map_of_alist ys)\<langle>x\<rangle> = None"
+definition has_key_alist :: "('a \<times> 'b) list \<Rightarrow> 'a \<Rightarrow> bool" where [rewrite]:
+  "has_key_alist xs a \<longleftrightarrow> (\<exists>p\<in>set xs. fst p = a)"
+
+lemma map_of_alist_nil [rewrite_back]:
+  "has_key_alist ys x \<longleftrightarrow> (map_of_alist ys)\<langle>x\<rangle> \<noteq> None"
 @proof @induct ys @qed
+setup {* add_rewrite_rule_cond @{thm map_of_alist_nil} [with_term "(map_of_alist ?ys)\<langle>?x\<rangle>"] *}
 
-section {* The unique *}
+lemma map_of_alist_some [forward]:
+  "(map_of_alist xs)\<langle>k\<rangle> = Some v \<Longrightarrow> (k, v) \<in> set xs"
+@proof @induct xs @qed
 
-definition THE_unique :: "('a \<Rightarrow> bool) \<Rightarrow> 'a option" where
-  "THE_unique P = (if (\<exists>!x. P x) then Some (THE x. P x) else None)"
-setup {* add_rewrite_rule @{thm THE_unique_def} *}
-
-theorem THE_uniqueI: "\<exists>!x. P x \<Longrightarrow> THE_unique P \<noteq> None \<and> P (the (THE_unique P))" by auto2
-setup {* add_forward_prfstep_cond @{thm THE_uniqueI} [with_term "THE_unique ?P"] *}
-
-theorem THE_unique_None: "\<not>(\<exists>!x. P x) \<Longrightarrow> THE_unique P = None" by auto2
-setup {* add_forward_prfstep_cond @{thm THE_unique_None} [with_term "THE_unique ?P"] *}
-
-theorem THE_unique_None': "\<not>(\<exists>x. P x) \<Longrightarrow> THE_unique P = None" by auto2
-setup {* add_forward_prfstep_cond @{thm THE_unique_None'} [with_term "THE_unique ?P"] *}
-
-theorem THE_unique_eq: "P a \<Longrightarrow> \<exists>!x. P x \<Longrightarrow> THE_unique P = Some a" by auto2
-setup {* add_forward_prfstep_cond @{thm THE_unique_eq} [with_term "THE_unique ?P"] *}
-
-theorem THE_uniqueD [resolve]: "THE_unique P = Some x \<Longrightarrow> P x"
-  by (metis THE_unique_def option.sel option.simps(3) theI')
-
-setup {* del_prfstep_thm @{thm THE_unique_def} *}
+lemma map_of_alist_nil':
+  "x \<in> set (map fst ys) \<longleftrightarrow> (map_of_alist ys)\<langle>x\<rangle> \<noteq> None"
+@proof @induct ys @qed
+setup {* add_rewrite_rule_cond @{thm map_of_alist_nil'} [with_term "(map_of_alist ?ys)\<langle>?x\<rangle>"] *}
     
-section {* Unique keys in an alist *}
+section {* Mapping defined by a set of key-value pairs *}
 
-definition unique_keys :: "(nat \<times> 'a) list \<Rightarrow> bool" where [rewrite]:
-  "unique_keys xs = (\<forall>m n. m < length xs \<longrightarrow> n < length xs \<longrightarrow> m \<noteq> n \<longrightarrow> fst (xs ! m) \<noteq> fst (xs ! n))"
-setup {* add_property_const @{term unique_keys} *}
-
-lemma unique_keysD:
-  "unique_keys xs \<Longrightarrow> m < length xs \<Longrightarrow> n < length xs \<Longrightarrow> m \<noteq> n \<Longrightarrow> fst (xs ! m) \<noteq> fst (xs ! n)" by auto2
-setup {* add_forward_prfstep_cond @{thm unique_keysD} [with_term "?xs ! ?m", with_term "?xs ! ?n"] *}
-setup {* del_prfstep_thm_eqforward @{thm unique_keys_def} *}
-
-definition has_key :: "('a \<times> 'b) list \<Rightarrow> 'a \<Rightarrow> bool" where
-  "has_key xs k = (\<exists>v'. (k, v') \<in># mset xs)"
-setup {* add_rewrite_rule @{thm has_key_def} *}
-
-theorem not_has_key [forward, backward2]:
-  "\<not>(has_key xs k) \<Longrightarrow> p \<in># mset xs \<Longrightarrow> k \<noteq> fst p" by auto2
-
-definition map_of_kv_set :: "('a \<times> 'b) set \<Rightarrow> ('a, 'b) map" where
-  "map_of_kv_set S = Map (\<lambda>a. THE_unique (\<lambda>b. (a, b) \<in> S))"
-setup {* add_rewrite_rule @{thm map_of_kv_set_def} *}
-
-setup {* add_gen_prfstep ("THE_unique_case",
-  [WithTerm @{term_pat "THE_unique (\<lambda>b. (?a, b) \<in> ?S)"},
-   CreateCase @{term_pat "\<exists>!b. (?a, b) \<in> ?S"}]) *}
-
-definition unique_keys_set :: "(nat \<times> 'a) set \<Rightarrow> bool" where
+definition unique_keys_set :: "('a \<times> 'b) set \<Rightarrow> bool" where [rewrite]:
   "unique_keys_set S = (\<forall>i x y. (i, x) \<in> S \<longrightarrow> (i, y) \<in> S \<longrightarrow> x = y)"
-setup {* add_rewrite_rule @{thm unique_keys_set_def} *}
+setup {* add_property_const @{term unique_keys_set} *}
 
-theorem unique_keys_imp [forward]:
-  "unique_keys_set S \<Longrightarrow> (i, x) \<in> S \<Longrightarrow> \<exists>!x. (i, x) \<in> S" by auto2
+lemma unique_keys_setD [forward]: "unique_keys_set S \<Longrightarrow> (i, x) \<in> S \<Longrightarrow> (i, y) \<in> S \<Longrightarrow> x = y" by auto2
+setup {* del_prfstep_thm_eqforward @{thm unique_keys_set_def} *}
 
-theorem map_of_kv_set_insert [rewrite]:
-  "unique_keys_set T \<Longrightarrow> \<forall>v. (k, v) \<notin> T \<Longrightarrow> map_of_kv_set (T \<union> { (k, v) }) = (map_of_kv_set T) {k \<rightarrow> v}"
+definition map_of_aset :: "('a \<times> 'b) set \<Rightarrow> ('a, 'b) map" where
+  "map_of_aset S = Map (\<lambda>a. if \<exists>b. (a, b) \<in> S then Some (THE b. (a, b) \<in> S) else None)"
+setup {* add_rewrite_rule @{thm map_of_aset_def} *}
+setup {* add_prfstep_check_req ("map_of_aset S", "unique_keys_set S") *}
+
+lemma map_of_asetI1 [rewrite]: "unique_keys_set S \<Longrightarrow> (a, b) \<in> S \<Longrightarrow> (map_of_aset S)\<langle>a\<rangle> = Some b"
+@proof @have "\<exists>b. (a, b) \<in> S" @have "\<exists>!b. (a, b) \<in> S" @qed
+
+lemma map_of_asetI2 [rewrite]: "\<forall>b. (a, b) \<notin> S \<Longrightarrow> (map_of_aset S)\<langle>a\<rangle> = None" by auto2
+
+lemma map_of_asetD1 [forward]: "(map_of_aset S)\<langle>a\<rangle> = None \<Longrightarrow> \<forall>b. (a, b) \<notin> S" by auto2
+
+lemma map_of_asetD2 [forward]:
+  "unique_keys_set S \<Longrightarrow> (map_of_aset S)\<langle>a\<rangle> = Some b \<Longrightarrow> (a, b) \<in> S" by auto2
+setup {* del_prfstep_thm @{thm map_of_aset_def} *}
+
+lemma map_of_aset_insert [rewrite]:
+  "unique_keys_set (S \<union> {(k, v)}) \<Longrightarrow> map_of_aset (S \<union> {(k, v)}) = (map_of_aset S) {k \<rightarrow> v}"
 @proof
-  @let "S = T \<union> { (k, v) }" @then
-  @have "T \<subseteq> S" @then @have "unique_keys_set S"
+  @let "M = map_of_aset S" "N = map_of_aset (S \<union> {(k, v)})"
+  @have (@rule) "\<forall>x. N\<langle>x\<rangle> = (M {k \<rightarrow> v}) \<langle>x\<rangle>" @with @case "M\<langle>x\<rangle> = None" @end
 @qed
 
-theorem map_of_kv_set_delete [rewrite]:
-  "unique_keys_set T \<Longrightarrow> (k, v) \<in> T \<Longrightarrow> map_of_kv_set (T - { (k, v) }) = delete_map k (map_of_kv_set T)"
-@proof
-  @let "S = T - { (k, v) }" @then
-  @have "S \<subseteq> T" @then @have "unique_keys_set S"
+lemma map_of_alist_to_aset [rewrite]:
+  "unique_keys_set (set xs) \<Longrightarrow> map_of_aset (set xs) = map_of_alist xs"
+@proof @induct xs @with
+  @subgoal "xs = x # xs'"
+    @have "set (x # xs') = set xs' \<union> {x}"
+  @endgoal @end
 @qed
 
-theorem map_of_kv_set_update [rewrite]:
-  "unique_keys_set T \<Longrightarrow> (k, v) \<in> T \<Longrightarrow>
-   map_of_kv_set ((T - { (k, v) }) \<union> { (k, v') }) = (map_of_kv_set T) {k \<rightarrow> v'}"
+lemma map_of_aset_delete [rewrite]:
+  "unique_keys_set S \<Longrightarrow> (k, v) \<in> S \<Longrightarrow> map_of_aset (S - {(k, v)}) = delete_map k (map_of_aset S)"
 @proof
-  @have "unique_keys_set (T - { (k, v) })" @then
-  @have "\<forall>x. (k, x) \<notin> T - { (k, v) }"
-@qed
-
-definition map_of_kv_list :: "('a \<times> 'b) list \<Rightarrow> ('a, 'b) map" where
-  "map_of_kv_list xs = map_of_kv_set (set xs)"
-setup {* add_rewrite_rule @{thm map_of_kv_list_def} *}
-
-theorem unique_keys_to_set [forward]:
-  "unique_keys xs \<Longrightarrow> unique_keys_set (set xs)"
-@proof
-  @let "S = set xs"
-  @have "\<forall>k x y. (k, x) \<in> S \<longrightarrow> (k, y) \<in> S \<longrightarrow> x = y" @with
-    @obtain i where "i < length xs" "xs ! i = (k, x)"
-    @obtain j where "j < length xs" "xs ! j = (k, y)"
+  @let "T = S - {(k, v)}" @then
+  @let "M = map_of_aset S" "N = map_of_aset T"
+  @have (@rule) "\<forall>x. N\<langle>x\<rangle> = (delete_map k M) \<langle>x\<rangle>" @with
+    @case "M\<langle>x\<rangle> = None" @case "x = k"
+    @obtain y where "M\<langle>x\<rangle> = Some y" @have "(x, y) \<in> T"
   @end
 @qed
 
-theorem unique_key_to_distinct [forward]: "unique_keys xs \<Longrightarrow> distinct xs"
-  using distinct_conv_nth unique_keys_def by fastforce
+lemma map_of_aset_update [rewrite]:
+  "unique_keys_set S \<Longrightarrow> (k, v) \<in> S \<Longrightarrow>
+   map_of_aset (S - {(k, v)} \<union> {(k, v')}) = (map_of_aset S) {k \<rightarrow> v'}" by auto2
 
-lemma map_of_kv_list_empty [backward]:
-  "[] = xs \<Longrightarrow> map_of_kv_list xs = empty_map" by auto2
+lemma map_of_alist_delete [rewrite]:
+  "set xs' = set xs - {x} \<Longrightarrow> unique_keys_set (set xs) \<Longrightarrow> x \<in> set xs \<Longrightarrow>
+   map_of_alist xs' = delete_map (fst x) (map_of_alist xs)"
+@proof @have "map_of_alist xs' = map_of_aset (set xs')" @qed
 
-theorem mset_update' [rewrite]:
-  "i < length ls \<Longrightarrow> mset (list_update ls i v) = {#v#} + (mset ls - {# ls ! i #})"
-  using mset_update by fastforce
+lemma map_of_alist_insert [rewrite]:
+  "set xs' = set xs \<union> {x} \<Longrightarrow> unique_keys_set (set xs') \<Longrightarrow>
+   map_of_alist xs' = (map_of_alist xs) {fst x \<rightarrow> snd x}"
+@proof @have "map_of_alist xs' = map_of_aset (set xs')" @qed
 
-theorem empty_list_to_empty_map [rewrite]:
-  "map_of_kv_list ([]::('a \<times> 'b) list) = empty_map" by auto2
+lemma map_of_alist_update [rewrite]:
+  "set xs' = set xs - {(k, v)} \<union> {(k, v')} \<Longrightarrow> unique_keys_set (set xs) \<Longrightarrow> (k, v) \<in> set xs \<Longrightarrow>
+   map_of_alist xs' = (map_of_alist xs) {k \<rightarrow> v'}"
+@proof @have "map_of_alist xs' = map_of_aset (set xs')" @qed
 
-theorem has_key_set [rewrite]:
-  "has_key xs k \<longleftrightarrow> (\<exists>v. (k, v) \<in> set xs)"
-@proof
-  @case "has_key xs k" @with
-    @obtain v where "(k, v) \<in># mset xs" @then @have "(k, v) \<in> set xs"
-  @end
-@qed
+section {* General update function on a mapping *}
 
-theorem has_key_to_map_none [rewrite_bidir]:
-  "unique_keys xs \<Longrightarrow> has_key xs k \<longleftrightarrow> (map_of_kv_list xs) \<langle>k\<rangle> \<noteq> None" by auto2
-setup {* del_prfstep_thm @{thm has_key_set} *}
+definition map_update_set :: "nat set \<Rightarrow> (nat \<Rightarrow> 'a) \<Rightarrow> (nat, 'a) map \<Rightarrow> (nat, 'a) map" where [rewrite]:
+  "map_update_set S f m = Map (\<lambda>i. if i \<in> S then Some (f i) else m\<langle>i\<rangle>)"
+
+fun map_update_set_impl :: "nat set \<Rightarrow> (nat \<Rightarrow> 'a) \<Rightarrow> (nat, 'a) map \<Rightarrow> nat \<Rightarrow> (nat, 'a) map" where
+  "map_update_set_impl S f m 0 = m"
+| "map_update_set_impl S f m (Suc k) =
+   (let m' = map_update_set_impl S f m k in
+      if k \<in> S then m' { k \<rightarrow> f k } else m')"
+setup {* fold add_rewrite_rule @{thms map_update_set_impl.simps} *}
+
+lemma map_update_set_impl_ind [rewrite]:
+  "map_update_set_impl S f m n =
+   Map (\<lambda>i. if i < n then if i \<in> S then Some (f i) else m\<langle>i\<rangle> else m\<langle>i\<rangle>)"
+@proof @induct n arbitrary m @qed
+
+lemma map_update_set_impl_correct [rewrite]:
+  "\<forall>i\<in>S. i < n \<Longrightarrow> map_update_set_impl S f m n = map_update_set S f m" by auto2
+
+definition map_constr_set :: "nat set \<Rightarrow> (nat \<Rightarrow> 'a) \<Rightarrow> (nat, 'a) map" where [rewrite]:
+  "map_constr_set S f = map_update_set S f empty_map"
 
 end
